Figuring out what are the correct statements to prove!

Bisimulation.v
@@ -5,65 +5,106 @@ Require Import SC.
 Require Import Util.
 Require Import Translation.
 
-Definition bisimilar (p : TSO_machine) (q : SC_machine) (f : nat -> nat) : Prop :=
-  let TSO_program := fst p in
-  let TSO_memory := snd p in
-  let SC_program := fst q in
-  let SC_memory := snd q in
-  let buf_size := fst (fst (fst TSO_program)) in
+Definition bisimilar_memory (TSO_memory : TSO.memory_model) (SC_memory : SC.memory_model) (B : nat) (f : nat -> nat) : Prop :=
+  let buf_size := fst (fst (fst TSO_memory)) in
   let local := snd (fst TSO_memory) in
   let TSOGS := snd TSO_memory in
   let TSO_mapping := snd (fst (fst TSO_memory)) in
   let SC_mapping := fst SC_memory in
   let SCGS := snd SC_memory in
-  let init := snd (fst (fst TSO_program)) in
-  let B := length init in
-  let init' := fst (fst (fst SC_program)) in
-  (translate_program TSO_program = SC_program) /\
+  (exists n, forall k, k >= n -> TSOGS k = None) /\ (* TSO memory is finite *)
+  (exists n, forall k, k >= n -> SCGS k = None) /\ (* SC memory is finite *)
   (forall n m k, TSO_mapping n = Some (m, k) -> SC_mapping n = Some (f m, k)) /\
   (forall n m, TSOGS n = Some m -> SCGS (f n) = Some m) /\
-  (init' = nil ->
-       (forall base offset value n, (nth_error (local true) n = Some (base, offset, value)) ->
-           exists BASES OFFSETS VALUES FRONT REAR SIZE front rear size,
-               (SC_mapping (B + LOOP_1_CONST) <> None /\
-                SC_mapping (B + FOUND_1_CONST) <> None /\
-                SC_mapping (B + RESULT_1_CONST) <> None /\
-                SC_mapping (B + BUFFER_1A_CONST) = Some (BASES, buf_size) /\
-                SC_mapping (B + BUFFER_1B_CONST) = Some (OFFSETS, buf_size) /\
-                SC_mapping (B + BUFFER_1C_CONST) = Some (VALUES, buf_size) /\
-                SC_mapping (B + FRONT_1_CONST) = Some (FRONT, buf_size) /\ SCGS FRONT = Some front /\
-                SC_mapping (B + REAR_1_CONST) = Some (REAR, buf_size) /\ SCGS REAR = Some rear /\
-                SC_mapping (B + SIZE_1_CONST) = Some (SIZE, buf_size) /\ SCGS SIZE = Some size /\
-                Nat.modulo (front + size - rear - 1) buf_size = 0 /\
-                SCGS SIZE = Some (length (local true)) /\
-                SCGS (BASES + (Nat.modulo (front + n) buf_size)) = Some base /\
-                SCGS (OFFSETS + (Nat.modulo (front + n) buf_size)) = Some offset /\
-                SCGS (VALUES + (Nat.modulo (front + n) buf_size)) = Some value
-               )
-       ) /\
-       (forall base offset value n, (nth_error (local true) n = Some (base, offset, value)) ->
-           exists BASES OFFSETS VALUES FRONT REAR SIZE front rear size,
-               (SC_mapping (B + LOOP_2_CONST) <> None /\
-                SC_mapping (B + FOUND_2_CONST) <> None /\
-                SC_mapping (B + RESULT_2_CONST) <> None /\
-                SC_mapping (B + BUFFER_2A_CONST) = Some (BASES, buf_size) /\
-                SC_mapping (B + BUFFER_2B_CONST) = Some (OFFSETS, buf_size) /\
-                SC_mapping (B + BUFFER_2C_CONST) = Some (VALUES, buf_size) /\
-                SC_mapping (B + FRONT_2_CONST) = Some (FRONT, buf_size) /\ SCGS FRONT = Some front /\
-                SC_mapping (B + REAR_2_CONST) = Some (REAR, buf_size) /\ SCGS REAR = Some rear /\
-                SC_mapping (B + SIZE_2_CONST) = Some (SIZE, buf_size) /\ SCGS SIZE = Some size /\
-                Nat.modulo (front + size - rear - 1) buf_size = 0 /\
-                SCGS SIZE = Some (length (local true)) /\
-                SCGS (BASES + (Nat.modulo (front + n) buf_size)) = Some base /\
-                SCGS (OFFSETS + (Nat.modulo (front + n) buf_size)) = Some offset /\
-                SCGS (VALUES + (Nat.modulo (front + n) buf_size)) = Some value
-               )
-       )
+  (forall base offset value n, (nth_error (local true) n = Some (base, offset, value)) ->
+      exists BASES OFFSETS VALUES FRONT REAR SIZE front rear size,
+        (SC_mapping (B + LOOP_1_CONST) <> None /\
+         SC_mapping (B + FOUND_1_CONST) <> None /\
+         SC_mapping (B + RESULT_1_CONST) <> None /\
+         SC_mapping (B + BUFFER_1A_CONST) = Some (BASES, buf_size) /\
+         SC_mapping (B + BUFFER_1B_CONST) = Some (OFFSETS, buf_size) /\
+         SC_mapping (B + BUFFER_1C_CONST) = Some (VALUES, buf_size) /\
+         SC_mapping (B + FRONT_1_CONST) = Some (FRONT, buf_size) /\ SCGS FRONT = Some front /\
+         SC_mapping (B + REAR_1_CONST) = Some (REAR, buf_size) /\ SCGS REAR = Some rear /\
+         SC_mapping (B + SIZE_1_CONST) = Some (SIZE, buf_size) /\ SCGS SIZE = Some size /\
+         Nat.modulo (front + size - rear - 1) buf_size = 0 /\
+         SCGS SIZE = Some (length (local true)) /\
+         SCGS (BASES + (Nat.modulo (front + n) buf_size)) = Some base /\
+         SCGS (OFFSETS + (Nat.modulo (front + n) buf_size)) = Some offset /\
+         SCGS (VALUES + (Nat.modulo (front + n) buf_size)) = Some value
+        )
+  ) /\
+  (forall base offset value n, (nth_error (local true) n = Some (base, offset, value)) ->
+      exists BASES OFFSETS VALUES FRONT REAR SIZE front rear size,
+        (SC_mapping (B + LOOP_2_CONST) <> None /\
+         SC_mapping (B + FOUND_2_CONST) <> None /\
+         SC_mapping (B + RESULT_2_CONST) <> None /\
+         SC_mapping (B + BUFFER_2A_CONST) = Some (BASES, buf_size) /\
+         SC_mapping (B + BUFFER_2B_CONST) = Some (OFFSETS, buf_size) /\
+         SC_mapping (B + BUFFER_2C_CONST) = Some (VALUES, buf_size) /\
+         SC_mapping (B + FRONT_2_CONST) = Some (FRONT, buf_size) /\ SCGS FRONT = Some front /\
+         SC_mapping (B + REAR_2_CONST) = Some (REAR, buf_size) /\ SCGS REAR = Some rear /\
+         SC_mapping (B + SIZE_2_CONST) = Some (SIZE, buf_size) /\ SCGS SIZE = Some size /\
+         Nat.modulo (front + size - rear - 1) buf_size = 0 /\
+         SCGS SIZE = Some (length (local true)) /\
+         SCGS (BASES + (Nat.modulo (front + n) buf_size)) = Some base /\
+         SCGS (OFFSETS + (Nat.modulo (front + n) buf_size)) = Some offset /\
+         SCGS (VALUES + (Nat.modulo (front + n) buf_size)) = Some value
+        )
   ).
 
-Definition psteps (p : SC_machine) (q : SC_machine) :=
-  exists l,
-  (length l >= 2 /\ hd_error l = Some p /\ hd_error (rev l) = Some q /\
-  (forall n a b, nth_error l n = Some a /\ nth_error l (S n) = Some b -> pstep a b)).
+Definition bisimilar (p : TSO_machine) (q : SC_machine) (f : nat -> nat) : Prop :=
+  let TSO_program := fst p in
+  let TSO_memory := snd p in
+  let SC_program := fst q in
+  let SC_memory := snd q in
+  let init := snd (fst (fst TSO_program)) in
+  let B := length init in
+  translate_program TSO_program = SC_program /\
+  bisimilar_memory TSO_memory SC_memory B f.
+
+Theorem forward_bisimulation : forall p p' q f,
+  TSO.pstep p p' -> bisimilar p q f -> (exists q', bisimilar p' q' f /\ psteps q q').
+Proof. intros. inversion H.
+  + subst. destruct q. destruct p. repeat (destruct p). destruct m. destruct mem. destruct mem'. repeat (destruct p0). repeat (destruct p).
+    inversion H3. subst. destruct H0. simpl in *. inversion H0. subst.
+    remember
+    (translate_vars xs buffer,
+     seq (translate s1 true (length (fst_list xs)) buffer) (flush_all true (length (fst_list xs)) buffer),
+     seq (translate s2 false (length (fst_list xs)) buffer) (flush_all false (length (fst_list xs)) buffer),
+     while tru (SPECIAL (length (fst_list xs)) [num 0]::= ZERO)) as answer_p.
+    unfold bisimilar_memory in H4. simpl in *. destruct H4. destruct H5. destruct H5.
+    remember (update_mapping x base size m, allocate x (x + size - 1) init g) as answer_m.
+    refine (ex_intro _ (answer_p, answer_m) _). subst. split.
+    ++ unfold bisimilar. simpl. split.
+      +++ intros. reflexivity.
+      +++ admit.
+    ++ admit.
+  + subst. generalize dependent q. induction H1 ; subst.
+    ++ intros. assert (TSO.pstep (buffer, nil, e, s2, mem) (buffer, nil, e', s2, mem')).
+       {apply TSO.ST_synchronize1 with (event:=event). auto. auto. }
+       assert (forall q : SC_machine,
+         bisimilar (buffer, nil, e, s2, mem) q f ->
+         exists q' : SC_machine,
+           bisimilar (buffer, nil, e', s2, mem') q' f /\
+           psteps q q'). {apply IHstep. auto. auto. } destruct q.
+       assert (bisimilar ((buffer, nil, e, s2), mem) (translate_program (buffer, nil, e, s2), m) f).
+       {split.
+          + reflexivity.
+          + simpl. destruct H0. simpl in H5. auto. }
+       apply H4 in H5. destruct H5. destruct H5. destruct H5. destruct x. simpl fst in *. 
+       simpl snd in *. subst.
+       refine (ex_intro _ (translate_program (buffer, nil, subst E e', s2), m0) _). split.
+      +++ split.
+        ++++ reflexivity.
+        ++++ simpl. simpl in H7. auto.
+      +++ unfold bisimilar in H0. destruct H0. simpl in *. subst.
+          assert (steps (seq (translate e true 0 buffer) (flush_all true 0 buffer)) (seq (translate e' true 0 buffer) (flush_all true 0 buffer))).
+          {apply psteps_inj_1 with (p:=(translate_vars nil buffer, seq (translate e true 0 buffer) (flush_all true 0 buffer),
+           seq (translate s2 false 0 buffer) (flush_all false 0 buffer), while tru (SPECIAL 0 [num 0]::= ZERO), m))
+           (q:=(translate_vars nil buffer, seq (translate e' true 0 buffer) (flush_all true 0 buffer),
+           seq (translate s2 false 0 buffer) (flush_all false 0 buffer), while tru (SPECIAL 0 [num 0]::= ZERO), m0)). apply H6. }
+          assert (steps (subst E e) (subst E e')).
+          {apply psteps_transports. apply steps_transitive with (q:=e') (event:=event). auto. apply steps_reflexive. }
 
 
